\documentclass[11pt]{article}
\usepackage{amsmath, amssymb}
\usepackage{amsfonts}
\usepackage{amsthm}
\usepackage{bbm}
\usepackage[algoruled]{algorithm2e}
\usepackage{a4wide}
\usepackage{verbatim}
\usepackage{latexsym}

\newcommand{\BigO}[1]{\ensuremath{\operatorname{O}\bigl(#1\bigr)}}
\newcommand{\Prob}[1]
{\mathbb{P}\left( #1 \right)}
\renewcommand{\vec}[1]{\mathbf{#1}}
\newcommand{\norm}[1]{\left\lVert#1\right\rVert}
\newcommand{\twopartdef}[4]
{
	\left\{
		\begin{array}{ll}
			#1 & \mbox{ } #2 \\
			#3 & \mbox{ } #4
		\end{array}
	\right.
}

\newtheoremstyle{break}
  {\topsep}{\topsep}%
  {\itshape}{}%
  {\bfseries}{}%
  {\newline}{}%
\theoremstyle{break}
\newtheorem{example}{Example}[section]
\newtheorem{thm}{Theorem}[section]
\newtheorem{lem}{Lemma}[section]
\newtheorem{definition}{Definition}[section]
\newtheorem{cor}{Corollary}[section]
\newtheorem{conj}{Conjecture}[section]
\newtheorem{condition}{Condition}[section]

\newcommand{\tn}{\widetilde{\nabla}_{n} }
\newcommand{\Z}{{\mathbb{Z}}}
\newcommand{\re}{{\mathbb{R}}}
\newcommand{\II}{{\mathbb{I}}}
\newcommand{\ep}{{\mathbb{E}}}
\newcommand{\FF}{{\mathcal{F}}}
\newcommand{\TT}{{\mathcal{T}}}
\newcommand{\phin}{\phig{n}}
\newcommand{\phig}[1]{\phi^{(#1)}}
\newcommand{\ol}[1]{\overline{#1}}
\newcommand{\eff}{{\rm eff}}

\begin{document}

\title{Large Deviations}

\date{\today}

\maketitle

\section{Cramer's Theorem}

\begin{definition}
\begin{equation}
\Lambda(t) = \log{M_x(t)} = \log{\ep{e^{tX}}}
\end{equation}
\end{definition}

\begin{definition}[LF Transform]

\begin{equation}
\Lambda^*(t) = \sup_{t\in\re}\{tx - \Lambda(t)\}
\end{equation}
\end{definition}

\begin{lem}[Properties of Rate Functions]
\leavevmode
\begin{enumerate}
\item \(\Lambda\) is convex. \(\Lambda^*\) is convex and a Rate Function:
\begin{enumerate}

\item \(\Lambda^*\) is Lower Semi-continuous 

\item If all level sets are compact, \(\Lambda^*\) is a Good Rate Function

\end{enumerate}

\item \(D_\Lambda = \{t: \Lambda(t) < \infty\}\), \(D_\Lambda^*\) likewise.

\begin{enumerate}
\item \(D_\Lambda = \{0\} \rightarrow \Lambda^* = 0\) 

\item \(\Lambda(t) < \infty \text{ for some } t>0 \rightarrow \bar{x}<\infty \text{ and } \forall x \geq \bar{x}\)
\begin{equation}
\Lambda^*(x) = \sup_{t\geq 0}\{tx - \Lambda(t)\}
\end{equation}
and it is non-decreasing for \(x\geq \bar{x}\)

\item \(\Lambda(t) < \infty \text{ for some } t<0 \rightarrow \bar{x}>-\infty \text{ and } \forall x \geq \bar{x}\)
\begin{equation}
\Lambda^*(x) = \sup_{t\leq 0}\{tx - \Lambda(t)\}
\end{equation}

and it is non-increasing for \(x\leq \bar{x}\)

\item \(\mid \bar{x} \mid < \infty \rightarrow \Lambda^*(\bar{x}) = 0\)

\item \(\inf_{x \in \re} \Lambda^*(\bar{x}) = 0\)
\end{enumerate}
\item \(\Lambda(\dot{•})\) is differentiable in \(D_\Lambda^{\dot{•}}\) with 
\begin{equation}
\Lambda^{'}(\eta) = \frac{1}{M(\eta)}\ep{X_1e^{\eta X_1}}
\end{equation}
and
\begin{equation}
\Lambda^{'}(\eta) = y \rightarrow \Lambda^* = \eta y - \Lambda(\eta)
\end{equation}
\end{enumerate}
\end{lem}

\begin{proof}
\leavevmode
\begin{enumerate}
\item We use Holder's inequality: given \(p,q \in [1,\infty] \text{ s.t } \frac{1}{p}+\frac{1}{q} = 1 \text{ } \forall f,g \text{ measurable}\): 
\begin{equation}
\norm{fg}_1 \leq \norm{f}_p \norm{g}_q
\end{equation}
\begin{eqnarray}
\Lambda(t\theta + (1-\theta)s) &= \log{\ep[{e^{(tX_1)\theta}e^{(sX_1)(1-\theta)}}}]\\
& \leq \log{\ep[{e^{(tX_1)\theta}]\ep[e^{(sX_1)(1-\theta)}}}]\\
&= \theta\log{\ep[e^{tX_1}]} +(1-\theta)\log{\ep[e^{sX_1}]}
\end{eqnarray}

\begin{eqnarray}
\Lambda^*(x_1\theta + (1-\theta)x_2) &= \sup\limits_{\lambda \in \re}\{\lambda(x_1\theta + (1-\theta)x_2) - \Lambda(\lambda)\} \\
& \leq \sup\limits_{\lambda \in \re}\{\lambda(x_1\theta -\theta\Lambda(\lambda)\} + \\ &   \sup\limits_{\lambda\in\re}\{(1-\theta)\lambda x_2) - (1-\theta)\Lambda(\lambda)\} \\
&= \theta\Lambda^*(x_1) + (1-\theta)\Lambda^*(x_2)
\end{eqnarray}
To prove that \(\Lambda^*\) is a Rate Function:
\begin{enumerate}

\item (Non-negativity) \(\Lambda(0) = \log{\ep[1]} = 0 \rightarrow \Lambda^*(x) \geq 0x - \Lambda(0) = 0\)
\item (Lower semi-continuity) FIx a sequence \(x_n \rightarrow x\). Then \(\forall \lambda\in\re\) 
\begin{eqnarray}
\liminf\limits_{x_n\rightarrow x} \Lambda^* \left(x_n\right) &\geq \liminf\limits_{x_n\rightarrow x} \left(\lambda x_n -\Lambda\left(\lambda\right) \right) \\
&=\lambda x - \Lambda\left(\lambda\right) \\
&\implies \liminf\limits_{x_n\rightarrow x} \Lambda^* \left(x_n\right) \geq \sup\limits_{\lambda \in \re} \left( \lambda x_n - \Lambda\lambda\right) \\
&= \Lambda^* \left(x\right)
\end{eqnarray}
\\
which is the definition of lower-semicontinuity.
\end{enumerate}

\item
\begin{enumerate}
\item \( D_\Lambda  := \{t:\Lambda\left(t\right)<\infty \}\) 
\(D_\Lambda = \{0\} \implies \Lambda\left(\lambda\right) \twopartdef{0}{\lambda = 0}{\infty}{\text{otherwise}}\)
\\
\(\implies \Lambda^*\left(x\right) = 0 \forall x\)

\item Let \( \Lambda\left(\lambda\right) = \log{M\left(\lambda\right)} < \infty \text{ for some } \lambda > 0\)

\begin{equation}
\implies \int_0^{\infty} xd\mu \leq \frac{\log\int_{\re} e^{\lambda x}d\mu }{ \lambda}
\end{equation}

\begin{eqnarray}
log\int_{\re} e^{\lambda x}d\mu &\geq \log\int_{0}^{\infty} e^{\lambda x}d\mu\\
&\geq \int_{\re} \log{e^{\lambda x}}d\mu\\
&= \lambda \int_{0}^{\infty} x d\mu \\
&\implies \bar{x}<\infty
\end{eqnarray}

\end{enumerate}

\end{enumerate}

\end{proof}


\end{document}